# Fibers of maps

```agda
{-# OPTIONS --without-K --exact-split #-}

module foundation.fibers-of-maps where

open import foundation-core.fibers-of-maps public

open import foundation.dependent-pair-types using (Σ; pair; pr1; pr2)
open import foundation.equivalences using (is-equiv; is-equiv-has-inverse; _≃_)
open import foundation.function-extensionality using (eq-htpy)
open import foundation.functions using (_∘_; id)
open import foundation.homotopies using (_~_)
open import foundation.identity-types using (refl)
open import foundation.universe-levels using (Level; UU)
```

## Properties

### When a product is taken over all fibers of a map, then we can equivalently take the product over the domain of that map.

```agda
map-reduce-Π-fib :
  {l1 l2 l3 : Level} {A : UU l1} {B : UU l2} (f : A → B)
  (C : (y : B) (z : fib f y) → UU l3) →
  ((y : B) (z : fib f y) → C y z) → ((x : A) → C (f x) (pair x refl))
map-reduce-Π-fib f C h x = h (f x) (pair x refl)

inv-map-reduce-Π-fib :
  {l1 l2 l3 : Level} {A : UU l1} {B : UU l2} (f : A → B)
  (C : (y : B) (z : fib f y) → UU l3) →
  ((x : A) → C (f x) (pair x refl)) → ((y : B) (z : fib f y) → C y z)
inv-map-reduce-Π-fib f C h .(f x) (pair x refl) = h x

issec-inv-map-reduce-Π-fib :
  {l1 l2 l3 : Level} {A : UU l1} {B : UU l2} (f : A → B)
  (C : (y : B) (z : fib f y) → UU l3) →
  ((map-reduce-Π-fib f C) ∘ (inv-map-reduce-Π-fib f C)) ~ id
issec-inv-map-reduce-Π-fib f C h = refl

isretr-inv-map-reduce-Π-fib' :
  {l1 l2 l3 : Level} {A : UU l1} {B : UU l2} (f : A → B)
  (C : (y : B) (z : fib f y) → UU l3) →
  (h : (y : B) (z : fib f y) → C y z) (y : B) →
  (inv-map-reduce-Π-fib f C ((map-reduce-Π-fib f C) h) y) ~ (h y)
isretr-inv-map-reduce-Π-fib' f C h .(f z) (pair z refl) = refl

isretr-inv-map-reduce-Π-fib :
  {l1 l2 l3 : Level} {A : UU l1} {B : UU l2} (f : A → B)
  (C : (y : B) (z : fib f y) → UU l3) →
  ((inv-map-reduce-Π-fib f C) ∘ (map-reduce-Π-fib f C)) ~ id
isretr-inv-map-reduce-Π-fib f C h =
  eq-htpy (λ y → eq-htpy (isretr-inv-map-reduce-Π-fib' f C h y))

is-equiv-map-reduce-Π-fib :
  {l1 l2 l3 : Level} {A : UU l1} {B : UU l2} (f : A → B) →
  (C : (y : B) (z : fib f y) → UU l3) →
  is-equiv (map-reduce-Π-fib f C)
is-equiv-map-reduce-Π-fib f C =
  is-equiv-has-inverse
    ( inv-map-reduce-Π-fib f C)
    ( issec-inv-map-reduce-Π-fib f C)
    ( isretr-inv-map-reduce-Π-fib f C)

reduce-Π-fib' :
  {l1 l2 l3 : Level} {A : UU l1} {B : UU l2} (f : A → B) →
  (C : (y : B) (z : fib f y) → UU l3) →
  ((y : B) (z : fib f y) → C y z) ≃ ((x : A) → C (f x) (pair x refl))
pr1 (reduce-Π-fib' f C) = map-reduce-Π-fib f C
pr2 (reduce-Π-fib' f C) = is-equiv-map-reduce-Π-fib f C

reduce-Π-fib :
  {l1 l2 l3 : Level} {A : UU l1} {B : UU l2} (f : A → B) →
  (C : B → UU l3) → ((y : B) → fib f y → C y) ≃ ((x : A) → C (f x))
reduce-Π-fib f C = reduce-Π-fib' f (λ y z → C y)
```
