# Functoriality of function types

```agda
{-# OPTIONS --without-K --exact-split #-}

module foundation.functoriality-function-types where

open import foundation.constant-maps using (const)
open import foundation.contractible-maps using
  ( is-equiv-is-contr-map; is-contr-map-is-equiv)
open import foundation.contractible-types using (center; eq-is-contr')
open import foundation.dependent-pair-types using (Σ; pair; pr1; pr2)
open import foundation.equivalences using
  ( is-equiv; is-equiv-has-inverse; map-inv-is-equiv; issec-map-inv-is-equiv;
    isretr-map-inv-is-equiv; _≃_; map-equiv; is-equiv-map-equiv)
open import foundation.functions using (postcomp; id; _∘_)
open import foundation.function-extensionality using (htpy-eq; eq-htpy)
open import foundation.functoriality-dependent-function-types using
  ( is-trunc-map-map-Π-is-trunc-map';
    is-trunc-map-is-trunc-map-map-Π')
open import foundation.homotopies using (htpy-right-whisk)
open import foundation.identity-types using (ap; refl)
open import foundation.truncated-maps using (is-trunc-map)
open import foundation.truncation-levels using (𝕋; neg-two-𝕋)
open import foundation.unit-type using (unit; star)
open import foundation.universe-levels using (Level; UU)
```

## Idea

```agda
is-trunc-map-postcomp-is-trunc-map :
  {l1 l2 l3 : Level} (k : 𝕋) (A : UU l3) {X : UU l1} {Y : UU l2} (f : X → Y) →
  is-trunc-map k f → is-trunc-map k (postcomp A f)
is-trunc-map-postcomp-is-trunc-map k A {X} {Y} f is-trunc-f =
  is-trunc-map-map-Π-is-trunc-map' k
    ( const A unit star)
    ( const unit (X → Y) f)
    ( const unit (is-trunc-map k f) is-trunc-f)

is-trunc-map-is-trunc-map-postcomp :
  {l1 l2 : Level} (k : 𝕋) {X : UU l1} {Y : UU l2} (f : X → Y) →
  ( {l3 : Level} (A : UU l3) → is-trunc-map k (postcomp A f)) →
  is-trunc-map k f
is-trunc-map-is-trunc-map-postcomp k {X} {Y} f is-trunc-post-f =
  is-trunc-map-is-trunc-map-map-Π' k
    ( const unit (X → Y) f)
    ( λ {l} {J} α → is-trunc-post-f {l} J)
    ( star)

abstract
  is-equiv-is-equiv-postcomp :
    {l1 l2 : Level} {X : UU l1} {Y : UU l2} (f : X → Y) →
    ({l3 : Level} (A : UU l3) → is-equiv (postcomp A f)) → is-equiv f
  is-equiv-is-equiv-postcomp {X = X} {Y = Y} f post-comp-equiv-f =
    is-equiv-is-contr-map
      ( is-trunc-map-is-trunc-map-postcomp neg-two-𝕋 f
        ( λ {l} A → is-contr-map-is-equiv (post-comp-equiv-f A)))

{- The following version of the same theorem works when X and Y are in the same
   universe. The condition of inducing equivalences by postcomposition is 
   simplified to that universe. -}

is-equiv-is-equiv-postcomp' :
  {l : Level} {X : UU l} {Y : UU l} (f : X → Y) →
  ((A : UU l) → is-equiv (postcomp A f)) → is-equiv f
is-equiv-is-equiv-postcomp'
  {l} {X} {Y} f is-equiv-postcomp-f =
  let sec-f = center (is-contr-map-is-equiv (is-equiv-postcomp-f Y) id)
  in
  is-equiv-has-inverse
    ( pr1 sec-f)
    ( htpy-eq (pr2 sec-f))
    ( htpy-eq
      ( ap ( pr1)
           ( eq-is-contr'
             ( is-contr-map-is-equiv (is-equiv-postcomp-f X) f)
             ( pair ((pr1 sec-f) ∘ f) (ap (λ t → t ∘ f) (pr2 sec-f)))
             ( pair id refl))))

abstract
  is-equiv-postcomp-is-equiv :
    {l1 l2 : Level} {X : UU l1} {Y : UU l2} (f : X → Y) → is-equiv f →
    ({l3 : Level} (A : UU l3) → is-equiv (postcomp A f))
  is-equiv-postcomp-is-equiv {X = X} {Y = Y} f is-equiv-f A =
    is-equiv-has-inverse 
      ( postcomp A (map-inv-is-equiv is-equiv-f))
      ( λ g → eq-htpy (htpy-right-whisk (issec-map-inv-is-equiv is-equiv-f) g))
      ( λ h → eq-htpy (htpy-right-whisk (isretr-map-inv-is-equiv is-equiv-f) h))

equiv-postcomp :
  {l1 l2 l3 : Level} {X : UU l1} {Y : UU l2} (A : UU l3) →
  (X ≃ Y) → (A → X) ≃ (A → Y)
pr1 (equiv-postcomp A e) = postcomp A (map-equiv e)
pr2 (equiv-postcomp A e) =
  is-equiv-postcomp-is-equiv (map-equiv e) (is-equiv-map-equiv e) A
```
